Merge `quantumlib_base` into `dev-kyle`.

GateHelpers.v
@@ -1,33 +1,32 @@
-Require Import QuantumLib.Quantum. 
+Require Import QuantumLib.Quantum.
+From Proof Require Import MatrixHelpers. 
 From Proof Require Import SwapHelpers.
 
 Definition abgate (U : Square 4) := U ⊗ I 2.
 Definition bcgate (U : Square 4) := I 2 ⊗ U.
 Definition acgate (U : Square 4) := swapbc × (abgate U) × swapbc.
+Definition ccu (U : Square 2) := control (control U).
 
 Lemma WF_abgate : forall (U : Square 4), WF_Matrix U -> WF_Matrix (abgate U).
 Proof.
-intros.
-apply WF_kron.
-reflexivity. reflexivity.
-apply H. apply WF_I.
+intros. solve_WF_matrix.
 Qed.
 
 Lemma WF_bcgate : forall (U : Square 4), WF_Matrix U -> WF_Matrix (bcgate U).
 Proof.
-intros.
-apply WF_kron.
-reflexivity. reflexivity.
-apply WF_I. apply H. 
+intros. solve_WF_matrix.
 Qed.
 
 Lemma WF_acgate : forall (U : Square 4), WF_Matrix U -> WF_Matrix (acgate U).
 Proof.
 intros.
-apply WF_mult. apply WF_mult.
+apply WF_mult. solve_WF_matrix.
 apply WF_swapbc.
-apply WF_abgate. apply H.
-apply WF_swapbc.
+Qed.
+
+Lemma WF_ccu : forall (U : Square 2), WF_Matrix U -> WF_Matrix (ccu U).
+Proof.
+intros. solve_WF_matrix.
 Qed.
 
 Lemma abgate_unitary : forall (U : Square 4), WF_Unitary U -> WF_Unitary (abgate U).
@@ -49,4 +48,10 @@ apply Mmult_unitary. apply Mmult_unitary.
 apply swapbc_unitary.
 apply abgate_unitary. apply H.
 apply swapbc_unitary.
+Qed.
+
+Lemma ccu_unitary : forall (U : Square 2), WF_Unitary U -> WF_Unitary (ccu U).
+Proof.
+intros.
+apply control_unitary. apply control_unitary. apply H.
 Qed.
