MatrixHelpers.v
@@ -1,53 +1,102 @@
 Require Import QuantumLib.Matrix.
 Require Import QuantumLib.Quantum.
+
+Ltac solve_WF_matrix := 
+    repeat (
+      progress (
+        try reflexivity;
+        try assumption; 
+        try apply WF_Zero;
+        try apply WF_I;
+        try apply WF_mult;
+        try apply WF_plus;
+        try apply WF_scale;
+        try apply WF_adjoint;
+        try apply WF_kron;
+        try apply WF_bra0;
+        try apply WF_bra1; 
+        try apply WF_qubit0; 
+        try apply WF_qubit1; 
+        try apply WF_braqubit0; 
+        try apply WF_braqubit1;
+        try apply WF_swap;
+        try apply WF_control;
+        try solve [intros; exfalso; auto]
+      )  
+    ).
+
+Definition diag2 (c1 c2 : C) : Square 2 :=
+    fun x y =>
+    match (x,y) with
+    | (0,0) => c1
+    | (1,1) => c2
+    | _ => C0
+    end.
+
+Lemma WF_diag2: forall (c1 c2 : C), WF_Matrix (diag2 c1 c2).
+Proof.
+unfold WF_Matrix.
+intros.
+destruct H.
+{
+    unfold diag2.
+    destruct x as [|x'].
+    contradict H.
+    lia.
+    destruct x' as [|x''].
+    contradict H.
+    lia. reflexivity.
+}
+{
+    unfold diag2.
+    destruct x as [|x'].
+    destruct y as [|y'].
+    contradict H.
+    lia. reflexivity.
+    destruct x' as [|x''].
+    destruct y as [|y'].
+    contradict H.
+    lia.
+    destruct y' as [|y''].
+    contradict H.
+    lia. reflexivity. reflexivity.
+}
+Qed.
+
 Lemma kron_0_vec2_equiv: forall (B C : Vector 2),
 WF_Matrix B -> WF_Matrix C -> ∣0⟩ ⊗ B = ∣0⟩ ⊗ C -> B = C.
 Proof.
 intros.
-cut ((B 0 0 = (∣0⟩ ⊗ B) 0 0 )%nat).
-cut ((B 1 0 = (∣0⟩ ⊗ B) 1 0 )%nat).
-cut ((C 0 0 = (∣0⟩ ⊗ C) 0 0 )%nat).
-cut ((C 1 0 = (∣0⟩ ⊗ C) 1 0 )%nat).
-intros.
-apply mat_equiv_eq.
-apply H. apply H0.
-by_cell.
-rewrite H5. rewrite H3. rewrite H1. reflexivity.
-rewrite H4. rewrite H2. rewrite H1. reflexivity.
-lca. lca. lca. lca.
+lma'.
+assert ((B 0 0 = (∣0⟩ ⊗ B) 0 0 )%nat). lca.
+assert ((C 0 0 = (∣0⟩ ⊗ C) 0 0 )%nat). lca.
+rewrite H2. rewrite H3. rewrite H1. reflexivity.
+assert ((B 1 0 = (∣0⟩ ⊗ B) 1 0 )%nat). lca.
+assert ((C 1 0 = (∣0⟩ ⊗ C) 1 0 )%nat). lca.
+rewrite H2. rewrite H3. rewrite H1. reflexivity.
 Qed.
 
 Lemma kron_1_vec2_equiv: forall (B C: Vector 2),
 WF_Matrix B -> WF_Matrix C -> ∣1⟩ ⊗ B = ∣1⟩ ⊗ C -> B = C.
 Proof.
 intros.
-cut ((B 0 0 = (∣1⟩ ⊗ B) 2 0 )%nat).
-cut ((B 1 0 = (∣1⟩ ⊗ B) 3 0 )%nat).
-cut ((C 0 0 = (∣1⟩ ⊗ C) 2 0 )%nat).
-cut ((C 1 0 = (∣1⟩ ⊗ C) 3 0 )%nat).
-intros.
-apply mat_equiv_eq.
-apply H. apply H0.
-by_cell.
-rewrite H5. rewrite H3. rewrite H1. reflexivity.
-rewrite H4. rewrite H2. rewrite H1. reflexivity.
-lca. lca. lca. lca.
+lma'.
+assert ((B 0 0 = (∣1⟩ ⊗ B) 2 0 )%nat). lca.
+assert ((C 0 0 = (∣1⟩ ⊗ C) 2 0 )%nat). lca.
+rewrite H2. rewrite H3. rewrite H1. reflexivity.
+assert ((B 1 0 = (∣1⟩ ⊗ B) 3 0 )%nat). lca.
+assert ((C 1 0 = (∣1⟩ ⊗ C) 3 0 )%nat). lca.
+rewrite H2. rewrite H3. rewrite H1. reflexivity.
 Qed.
 
 Lemma WF_ket0bra1: WF_Matrix ∣0⟩⟨1∣.
 Proof.
-apply WF_mult.
-apply WF_qubit0.
-apply WF_adjoint.
-apply WF_qubit1.
+solve_WF_matrix.
 Qed.
 
 Lemma WF_ket1bra0: WF_Matrix ∣1⟩⟨0∣.
 Proof.
-apply WF_mult.
-apply WF_qubit1.
-apply WF_adjoint.
-apply WF_qubit0.
+solve_WF_matrix.
 Qed.
 
 Lemma WF_blockmatrix: forall (P00 P01 P10 P11: Square 2), 
@@ -55,25 +104,7 @@ WF_Matrix P00 -> WF_Matrix P01 -> WF_Matrix P10 -> WF_Matrix P11 ->
 WF_Matrix (∣0⟩⟨0∣ ⊗ P00 .+ ∣0⟩⟨1∣ ⊗ P01 .+ ∣1⟩⟨0∣ ⊗ P10 .+ ∣1⟩⟨1∣ ⊗ P11).
 Proof.
 intros.
-apply WF_plus.
-apply WF_plus.
-apply WF_plus.
-apply WF_kron.
-ring. ring.
-apply WF_braqubit0.
-apply H.
-apply WF_kron.
-ring. ring.
-apply WF_ket0bra1.
-apply H0.
-apply WF_kron.
-ring. ring.
-apply WF_ket1bra0.
-apply H1.
-apply WF_kron.
-ring. ring.
-apply WF_braqubit1.
-apply H2.
+solve_WF_matrix.
 Qed.
 
 Lemma block_multiply: forall (U V: Square 4) (P00 P01 P10 P11 Q00 Q01 Q10 Q11: Square 2), 
@@ -83,45 +114,11 @@ U = ∣0⟩⟨0∣ ⊗ P00 .+ ∣0⟩⟨1∣ ⊗ P01 .+ ∣1⟩⟨0∣ ⊗ P10 .
 V = ∣0⟩⟨0∣ ⊗ Q00 .+ ∣0⟩⟨1∣ ⊗ Q01 .+ ∣1⟩⟨0∣ ⊗ Q10 .+ ∣1⟩⟨1∣ ⊗ Q11 -> 
 U × V = ∣0⟩⟨0∣ ⊗ (P00 × Q00 .+ P01 × Q10) .+ ∣0⟩⟨1∣ ⊗ (P00 × Q01 .+ P01×Q11) .+ ∣1⟩⟨0∣ ⊗ (P10×Q00 .+ P11 × Q10) .+ ∣1⟩⟨1∣ ⊗ (P10 × Q01 .+ P11 × Q11).
 Proof.
-intros U V P00 P01 P10 P11 Q00 Q01 Q10 Q11 H1 H2 H3 H4 H5 H6 H7 H8 H9 H10.
-rewrite H9. rewrite H10.
-apply mat_equiv_eq.
-{
-    apply WF_mult.
-    apply WF_blockmatrix.
-    apply H1. apply H2. apply H3. apply H4.
-    apply WF_blockmatrix.
-    apply H5. apply H6. apply H7. apply H8.
-}
-{
-    apply WF_blockmatrix.
-    apply WF_plus.
-    apply WF_mult.
-    apply H1. apply H5.
-    apply WF_mult.
-    apply H2. apply H7.
-    apply WF_plus.
-    apply WF_mult.
-    apply H1. apply H6.
-    apply WF_mult.
-    apply H2. apply H8.  
-    apply WF_plus.
-    apply WF_mult.
-    apply H3. apply H5.
-    apply WF_mult.
-    apply H4. apply H7.  
-    apply WF_plus.
-    apply WF_mult.
-    apply H3. apply H6.
-    apply WF_mult.
-    apply H4. apply H8.     
-}
-{
-    unfold Mmult. unfold Mplus. unfold kron.
-    by_cell.
-    lca. lca. lca. lca. lca. lca. lca. lca.
-    lca. lca. lca. lca. lca. lca. lca. lca.
-}
+intros.
+rewrite H7. rewrite H8.
+lma'.
+solve_WF_matrix.
+solve_WF_matrix.
 Qed.
 
 Lemma block_equalities: forall (U V: Square 4) (P00 P01 P10 P11 Q00 Q01 Q10 Q11: Square 2), 
@@ -131,129 +128,75 @@ U = ∣0⟩⟨0∣ ⊗ P00 .+ ∣0⟩⟨1∣ ⊗ P01 .+ ∣1⟩⟨0∣ ⊗ P10 .
 V = ∣0⟩⟨0∣ ⊗ Q00 .+ ∣0⟩⟨1∣ ⊗ Q01 .+ ∣1⟩⟨0∣ ⊗ Q10 .+ ∣1⟩⟨1∣ ⊗ Q11 -> 
 U = V -> P00 = Q00 /\ P01 = Q01 /\ P10 = Q10 /\ P11 = Q11.
 Proof.
-intros U V P00 P01 P10 P11 Q00 Q01 Q10 Q11 H1 H2 H3 H4 H5 H6 H7 H8 H9 H10 H11.
+intros U V P00 P01 P10 P11 Q00 Q01 Q10 Q11 WF_P00 WF_P01 WF_P10 WF_P11 WF_Q00 WF_Q01 WF_Q10 WF_Q11
+def_U def_V H.
 split.
 {
-    apply mat_equiv_eq.
-    apply H1. apply H5.
-    by_cell.
-    cut (P00 0%nat 0%nat = U 0%nat 0%nat).
-    cut (Q00 0%nat 0%nat = V 0%nat 0%nat).
-    intros H12 H13.
-    rewrite H12. rewrite H13. rewrite H11. reflexivity.
-    rewrite H10. lca.
-    rewrite H9. lca.
-    cut (P00 0%nat 1%nat = U 0%nat 1%nat).
-    cut (Q00 0%nat 1%nat = V 0%nat 1%nat).
-    intros H12 H13.
-    rewrite H12. rewrite H13. rewrite H11. reflexivity.
-    rewrite H10. lca.
-    rewrite H9. lca.
-    cut (P00 1%nat 0%nat = U 1%nat 0%nat).
-    cut (Q00 1%nat 0%nat = V 1%nat 0%nat).
-    intros H12 H13.
-    rewrite H12. rewrite H13. rewrite H11. reflexivity.
-    rewrite H10. lca.
-    rewrite H9. lca.
-    cut (P00 1%nat 1%nat = U 1%nat 1%nat).
-    cut (Q00 1%nat 1%nat = V 1%nat 1%nat).
-    intros H12 H13.
-    rewrite H12. rewrite H13. rewrite H11. reflexivity.
-    rewrite H10. lca.
-    rewrite H9. lca.
+    lma'.
+    assert (peq: P00 0%nat 0%nat = U 0%nat 0%nat). rewrite def_U. lca.
+    assert (qeq: Q00 0%nat 0%nat = V 0%nat 0%nat). rewrite def_V. lca.
+    rewrite peq. rewrite qeq. rewrite H. reflexivity.
+    assert (peq: P00 0%nat 1%nat = U 0%nat 1%nat). rewrite def_U. lca.
+    assert (qeq: Q00 0%nat 1%nat = V 0%nat 1%nat). rewrite def_V. lca.
+    rewrite peq. rewrite qeq. rewrite H. reflexivity.
+    assert (peq: P00 1%nat 0%nat = U 1%nat 0%nat). rewrite def_U. lca.
+    assert (qeq: Q00 1%nat 0%nat = V 1%nat 0%nat). rewrite def_V. lca.
+    rewrite peq. rewrite qeq. rewrite H. reflexivity.
+    assert (peq: P00 1%nat 1%nat = U 1%nat 1%nat). rewrite def_U. lca.
+    assert (qeq: Q00 1%nat 1%nat = V 1%nat 1%nat). rewrite def_V. lca.
+    rewrite peq. rewrite qeq. rewrite H. reflexivity.
 }
 split.
 {
-    apply mat_equiv_eq.
-    apply H2. apply H6.
-    by_cell.
-    cut (P01 0%nat 0%nat = U 0%nat 2%nat).
-    cut (Q01 0%nat 0%nat = V 0%nat 2%nat).
-    intros H12 H13.
-    rewrite H12. rewrite H13. rewrite H11. reflexivity.
-    rewrite H10. lca.
-    rewrite H9. lca.
-    cut (P01 0%nat 1%nat = U 0%nat 3%nat).
-    cut (Q01 0%nat 1%nat = V 0%nat 3%nat).
-    intros H12 H13.
-    rewrite H12. rewrite H13. rewrite H11. reflexivity.
-    rewrite H10. lca.
-    rewrite H9. lca.
-    cut (P01 1%nat 0%nat = U 1%nat 2%nat).
-    cut (Q01 1%nat 0%nat = V 1%nat 2%nat).
-    intros H12 H13.
-    rewrite H12. rewrite H13. rewrite H11. reflexivity.
-    rewrite H10. lca.
-    rewrite H9. lca.
-    cut (P01 1%nat 1%nat = U 1%nat 3%nat).
-    cut (Q01 1%nat 1%nat = V 1%nat 3%nat).
-    intros H12 H13.
-    rewrite H12. rewrite H13. rewrite H11. reflexivity.
-    rewrite H10. lca.
-    rewrite H9. lca.
-} 
+    lma'.
+    assert (peq: P01 0%nat 0%nat = U 0%nat 2%nat). rewrite def_U. lca.
+    assert (qeq: Q01 0%nat 0%nat = V 0%nat 2%nat). rewrite def_V. lca.
+    rewrite peq. rewrite qeq. rewrite H. reflexivity.
+    assert (peq: P01 0%nat 1%nat = U 0%nat 3%nat). rewrite def_U. lca.
+    assert (qeq: Q01 0%nat 1%nat = V 0%nat 3%nat). rewrite def_V. lca.
+    rewrite peq. rewrite qeq. rewrite H. reflexivity.
+    assert (peq: P01 1%nat 0%nat = U 1%nat 2%nat). rewrite def_U. lca.
+    assert (qeq: Q01 1%nat 0%nat = V 1%nat 2%nat). rewrite def_V. lca.
+    rewrite peq. rewrite qeq. rewrite H. reflexivity.
+    assert (peq: P01 1%nat 1%nat = U 1%nat 3%nat). rewrite def_U. lca.
+    assert (qeq: Q01 1%nat 1%nat = V 1%nat 3%nat). rewrite def_V. lca.
+    rewrite peq. rewrite qeq. rewrite H. reflexivity.
+}
 split.
 {
-    apply mat_equiv_eq.
-    apply H3. apply H7.
-    by_cell.
-    cut (P10 0%nat 0%nat = U 2%nat 0%nat).
-    cut (Q10 0%nat 0%nat = V 2%nat 0%nat).
-    intros H12 H13.
-    rewrite H12. rewrite H13. rewrite H11. reflexivity.
-    rewrite H10. lca.
-    rewrite H9. lca.
-    cut (P10 0%nat 1%nat = U 2%nat 1%nat).
-    cut (Q10 0%nat 1%nat = V 2%nat 1%nat).
-    intros H12 H13.
-    rewrite H12. rewrite H13. rewrite H11. reflexivity.
-    rewrite H10. lca.
-    rewrite H9. lca.
-    cut (P10 1%nat 0%nat = U 3%nat 0%nat).
-    cut (Q10 1%nat 0%nat = V 3%nat 0%nat).
-    intros H12 H13.
-    rewrite H12. rewrite H13. rewrite H11. reflexivity.
-    rewrite H10. lca.
-    rewrite H9. lca.
-    cut (P10 1%nat 1%nat = U 3%nat 1%nat).
-    cut (Q10 1%nat 1%nat = V 3%nat 1%nat).
-    intros H12 H13.
-    rewrite H12. rewrite H13. rewrite H11. reflexivity.
-    rewrite H10. lca.
-    rewrite H9. lca.
+    lma'.
+    assert (peq: P10 0%nat 0%nat = U 2%nat 0%nat). rewrite def_U. lca.
+    assert (qeq: Q10 0%nat 0%nat = V 2%nat 0%nat). rewrite def_V. lca.
+    rewrite peq. rewrite qeq. rewrite H. reflexivity.
+    assert (peq: P10 0%nat 1%nat = U 2%nat 1%nat). rewrite def_U. lca.
+    assert (qeq: Q10 0%nat 1%nat = V 2%nat 1%nat). rewrite def_V. lca.
+    rewrite peq. rewrite qeq. rewrite H. reflexivity.
+    assert (peq: P10 1%nat 0%nat = U 3%nat 0%nat). rewrite def_U. lca.
+    assert (qeq: Q10 1%nat 0%nat = V 3%nat 0%nat). rewrite def_V. lca.
+    rewrite peq. rewrite qeq. rewrite H. reflexivity.
+    assert (peq: P10 1%nat 1%nat = U 3%nat 1%nat). rewrite def_U. lca.
+    assert (qeq: Q10 1%nat 1%nat = V 3%nat 1%nat). rewrite def_V. lca.
+    rewrite peq. rewrite qeq. rewrite H. reflexivity.
 }
 {
-    apply mat_equiv_eq.
-    apply H4. apply H8.
-    by_cell.
-    cut (P11 0%nat 0%nat = U 2%nat 2%nat).
-    cut (Q11 0%nat 0%nat = V 2%nat 2%nat).
-    intros H12 H13.
-    rewrite H12. rewrite H13. rewrite H11. reflexivity.
-    rewrite H10. lca.
-    rewrite H9. lca.
-    cut (P11 0%nat 1%nat = U 2%nat 3%nat).
-    cut (Q11 0%nat 1%nat = V 2%nat 3%nat).
-    intros H12 H13.
-    rewrite H12. rewrite H13. rewrite H11. reflexivity.
-    rewrite H10. lca.
-    rewrite H9. lca.
-    cut (P11 1%nat 0%nat = U 3%nat 2%nat).
-    cut (Q11 1%nat 0%nat = V 3%nat 2%nat).
-    intros H12 H13.
-    rewrite H12. rewrite H13. rewrite H11. reflexivity.
-    rewrite H10. lca.
-    rewrite H9. lca.
-    cut (P11 1%nat 1%nat = U 3%nat 3%nat).
-    cut (Q11 1%nat 1%nat = V 3%nat 3%nat).
-    intros H12 H13.
-    rewrite H12. rewrite H13. rewrite H11. reflexivity.
-    rewrite H10. lca.
-    rewrite H9. lca.
+    lma'.
+    assert (peq: P11 0%nat 0%nat = U 2%nat 2%nat). rewrite def_U. lca.
+    assert (qeq: Q11 0%nat 0%nat = V 2%nat 2%nat). rewrite def_V. lca.
+    rewrite peq. rewrite qeq. rewrite H. reflexivity.
+    assert (peq: P11 0%nat 1%nat = U 2%nat 3%nat). rewrite def_U. lca.
+    assert (qeq: Q11 0%nat 1%nat = V 2%nat 3%nat). rewrite def_V. lca.
+    rewrite peq. rewrite qeq. rewrite H. reflexivity.
+    assert (peq: P11 1%nat 0%nat = U 3%nat 2%nat). rewrite def_U. lca.
+    assert (qeq: Q11 1%nat 0%nat = V 3%nat 2%nat). rewrite def_V. lca.
+    rewrite peq. rewrite qeq. rewrite H. reflexivity.
+    assert (peq: P11 1%nat 1%nat = U 3%nat 3%nat). rewrite def_U. lca.
+    assert (qeq: Q11 1%nat 1%nat = V 3%nat 3%nat). rewrite def_V. lca.
+    rewrite peq. rewrite qeq. rewrite H. reflexivity.
 }
 Qed.
 
 Lemma neq_implies_const_div_neq: forall (i j m: nat), (m <> 0)%nat -> (i <> j)%nat -> (i / m <> j / m)%nat \/ (i mod m <> j mod m)%nat.
+(* Thanks Kyle *)
 Proof.
   intros.
   assert (H1 : ({i mod m = j mod m} + {i mod m <> j mod m})%nat).
@@ -276,84 +219,81 @@ Qed.
 
 Lemma kron_I {n m : nat} : (n > 0)%nat -> (m > 0)%nat -> I n ⊗ I m = I (n * m).
 Proof.
-  intros.
-  apply mat_equiv_eq.
-  apply WF_kron. reflexivity. reflexivity. apply WF_I. apply WF_I.
-  apply WF_I.
-  by_cell.
-  destruct (Nat.eq_dec i j) as [Heq | Hneq].
-  {
+intros.
+lma'.
+destruct (eq_nat_decide i j) as [Heq | Hneq].
+{
+    apply eq_nat_is_eq in Heq.
     rewrite Heq.
-    unfold I at 3.
-    rewrite Nat.eqb_refl; simpl.
+    unfold I at 3, kron.
+    rewrite Nat.eqb_refl.
+    simpl.
     destruct (j <? n * m) eqn:Hlt.
     {
-      unfold kron.
-      unfold I.
-      rewrite Nat.eqb_refl; rewrite Nat.eqb_refl; simpl.
-      rewrite Nat.ltb_lt in Hlt.
-      assert ((j / m <? n) = true).
-      {
-        apply Nat.ltb_lt.
-        apply Nat.div_lt_upper_bound.
-        lia.
-        rewrite Nat.mul_comm.
-        assumption.
-      }
-      assert ((j mod m <? m) = true).
-      {
-        apply Nat.ltb_lt.
-        apply Nat.mod_upper_bound.
-        lia.
-      }
-      rewrite H1; rewrite H2.
-      lca.
+        unfold I.
+        rewrite Nat.eqb_refl. rewrite Nat.eqb_refl. simpl.
+        assert ((j / m <? n) = true). 
+        {
+            apply Nat.ltb_lt. apply Nat.ltb_lt in Hlt.
+            apply Nat.div_lt_upper_bound. lia.
+            rewrite Nat.mul_comm.
+            apply Hlt.
+        }
+        rewrite H1.
+        assert ((j mod m <? m) = true).
+        {
+            apply Nat.ltb_lt.
+            apply Nat.mod_upper_bound. lia. 
+        }
+        rewrite H2.
+        lca.
     }
     {
-      apply Nat.ltb_ge in Hlt.
-      unfold kron; unfold I.
-      cut ((j / m <? n) = false).
-      intros.
-      rewrite H1.
-      rewrite Coq.Bool.Bool.andb_false_r.
-      lca.
-      apply Nat.ltb_ge.
-      rewrite <- Nat.div_mul with (a := n) (b := m). 2: lia.
-      apply Nat.div_le_mono. lia.
-      lia.
+        apply Nat.ltb_ge in Hlt.
+        unfold I at 1.
+        assert ((n = (n * m) / m)%nat). rewrite Nat.div_mul; try lia.
+        assert ((j / m <? n) = false).
+        {
+            apply Nat.ltb_ge.
+            rewrite H1.
+            apply Nat.div_le_mono. lia.
+            apply Hlt.
+        }
+        rewrite H2.
+        rewrite Coq.Bool.Bool.andb_false_r.
+        lca.
     }
-  }
-  {
+}
+{
+    rewrite eq_nat_is_eq in Hneq.
     unfold I at 3.
-    assert ((i =? j) && (i <? n * m) = false).
+    assert ((i =? j) = false).
     {
-      rewrite <- Nat.eqb_neq in Hneq.
-      rewrite Hneq.
-      apply Coq.Bool.Bool.andb_false_l.
+        apply Nat.eqb_neq.
+        assumption.
+    }
+    assert ((i =? j) && (i <? n * m) = false). 
+    {
+        rewrite H1.
+        apply Coq.Bool.Bool.andb_false_l.
     }
     rewrite H1.
-    unfold kron; unfold I.
+    unfold kron.
+    unfold I.
     assert ((i / m =? j / m) = false \/ (i mod m =? j mod m) = false).
     {
-      rewrite Nat.eqb_neq; rewrite Nat.eqb_neq.
-      apply neq_implies_const_div_neq.
-      lia.
-      assumption.
+        rewrite Nat.eqb_neq. rewrite Nat.eqb_neq.
+        apply neq_implies_const_div_neq. lia.
+        assumption.
     }
     assert (((i / m =? j / m) && (i / m <? n)) = false \/ (i mod m =? j mod m) && (i mod m <? m) = false).
     {
-      destruct H2.
-      rewrite H2.
-      left.
-      apply Coq.Bool.Bool.andb_false_l.
-      right.
-      rewrite H2.
-      apply Coq.Bool.Bool.andb_false_l.
+        destruct H3.
+        rewrite H3. left. apply Coq.Bool.Bool.andb_false_l.
+        rewrite H3. right. apply Coq.Bool.Bool.andb_false_l.
     }
-    destruct H2.
-    rewrite H2.
-    lca.
-    rewrite H2.
-    lca.
-  }
+    destruct H4.
+    rewrite H4. lca.
+    rewrite H4. lca.
+}
 Qed.
