Swaps.v
@@ -1,124 +1,112 @@
 Require Import QuantumLib.Quantum.
 From Proof Require Import SwapHelpers.
 From Proof Require Import GateHelpers.
+From Proof Require Import MatrixHelpers.
 From Proof Require Import SwapProperty.
 Lemma a10 : forall (a b : Vector 2),
   WF_Matrix a -> WF_Matrix b -> 
   swap × (a ⊗ b) = b ⊗ a.
 Proof.
   intros.
-  apply mat_equiv_eq.
-  apply WF_mult.
-  apply WF_swap.
-  apply WF_kron. reflexivity. reflexivity. apply H. apply H0.
-  apply WF_kron. reflexivity. reflexivity. apply H0. apply H.
-  by_cell.
-  lca. lca. lca. lca.
+  lma'.
 Qed.
 
 Lemma a11 : forall (A B : Square 2),
   WF_Matrix A -> WF_Matrix B ->
   swap × (A ⊗ B) × swap = B ⊗ A.
 Proof.
-  intros.
-  apply mat_equiv_eq.
-  apply WF_mult. apply WF_mult.
-  apply WF_swap.
-  apply WF_kron. reflexivity. reflexivity. apply H. apply H0.
-  apply WF_swap.
-  apply WF_kron. reflexivity. reflexivity. apply H0. apply H.
-  by_cell.
-  lca. lca. lca. lca. lca. lca. lca. lca.
-  lca. lca. lca. lca. lca. lca. lca. lca.
+apply swap_2q.
 Qed.
 
 Lemma a12 : forall (U : Square 4),
   WF_Matrix U -> swapab × acgate U × swapab = bcgate U.
 Proof.
 intros.
-apply mat_equiv_eq.
-apply WF_mult. apply WF_mult. apply WF_swapab. apply WF_acgate. apply H. apply WF_swapab.
-apply WF_bcgate. apply H.
 unfold acgate. unfold swapbc. unfold abgate.
-rewrite swap_helper.
+rewrite swap_helper. 2: apply H.
 fold swapab.
 rewrite <- Mmult_assoc.
 rewrite <- Mmult_assoc with (A:= swapab) (B:= swapab) (C:=(I 2 ⊗ U)).
 rewrite swapab_inverse. 
-rewrite Mmult_1_l.
 rewrite Mmult_assoc.
-rewrite swapab_inverse at 1.
-rewrite Mmult_1_r.
+rewrite Mmult_1_l.
+rewrite swapab_inverse at 1. 2: solve_WF_matrix.
+rewrite Mmult_1_r. 2: solve_WF_matrix.
 unfold bcgate.
-apply mat_equiv_refl.
-apply WF_kron. reflexivity. reflexivity. apply WF_I. apply H.
-apply WF_kron. reflexivity. reflexivity. apply WF_I. apply H.
-apply H.
+reflexivity.
 Qed.
 
-(* 
-(* TODO: This proof has changed between versions. Is it better to outline the steps in the proof, 
-if lma is sufficient to verify the lemma? *)
-Lemma a10_1 : forall (D: Unitary 2), SWAPAB × CCU (D) × SWAPAB  == CCU (D).
-Proof.
-unfold CCU, Diag2.
-lma.
-Qed.
-
-Lemma a10_2 : forall (c1 : C), SWAPBC × CCU (Diag2 1 c1) × SWAPBC == CCU (Diag2 1 c1).
-Proof.
-unfold CCU, Diag2.
-lma.
-Qed.
-
-Lemma a10_3 : forall (c1 : C), SWAPAC × CCU (Diag2 1 c1) × SWAPAC == CCU (Diag2 1 c1).
+Lemma a10_1 : forall (D: Square 2), WF_Matrix D -> swapab × ccu (D) × swapab  = ccu (D).
 Proof.
 intros.
-assert (Help : CCU (Diag2 1 c1) == 
-  (∣0⟩ × ∣0⟩†) ⊗ I 4 + (∣1⟩ × ∣1⟩†) ⊗ CU (Diag2 1 c1)).
+lma'.
+apply WF_mult. apply WF_mult. apply WF_swapab. apply WF_ccu. apply H. apply WF_swapab.
+apply WF_ccu. apply H.
+Qed.
+
+Lemma a10_2 : forall (c1 : C), swapbc × ccu (diag2 1 c1) × swapbc = ccu (diag2 1 c1).
+Proof.
+intros.
+lma'.
+apply WF_mult. apply WF_mult. apply WF_swapbc. apply WF_ccu. apply WF_diag2. apply WF_swapbc.
+apply WF_ccu. apply WF_diag2.
+Qed.
+
+Lemma a10_3 : forall (c1 : C), swapac × ccu (diag2 1 c1) × swapac = ccu (diag2 1 c1).
+Proof.
+intros.
+assert (Help : ccu (diag2 1 c1) =
+  ∣0⟩⟨0∣ ⊗ I 4 .+ ∣1⟩⟨1∣ ⊗ control (diag2 1 c1)).
 {
-  unfold CCU, CU, Diag2. lma.
+  lma'.
+  apply WF_ccu. apply WF_diag2.
+  solve_WF_matrix. apply WF_diag2.
+  unfold ccu, diag2, control.
+  lca.
 }
 rewrite Help; clear Help.
-rewrite Mmult_plus_dist_l.
-repeat rewrite Mmult_plus_dist_r.
-assert (Help : CU (Diag2 1 c1) == (∣0⟩ × ∣0⟩†) ⊗ I 2 + (∣1⟩ × ∣1⟩†) ⊗ Diag2 1 c1).
+rewrite Mmult_plus_distr_l.
+repeat rewrite Mmult_plus_distr_r.
+assert (Help : control (diag2 1 c1) = ∣0⟩⟨0∣ ⊗ I 2 .+ ∣1⟩⟨1∣ ⊗ diag2 1 c1).
 {
-  unfold CU, Diag2. lma.
+  lma'.
+  apply WF_control. apply WF_diag2.
+  solve_WF_matrix. apply WF_diag2. 
+  unfold control, diag2.  lca.
 }
 rewrite Help; clear Help.
-rewrite kron_plus_dist_l.
-rewrite Mmult_plus_dist_l.
-repeat rewrite Mmult_plus_dist_r.
-assert (Main1 : SWAPAC × 
-  ((∣0⟩ × ∣0⟩†) ⊗ I 4) × SWAPAC ==
-  I 4 ⊗ (∣0⟩ × ∣0⟩†)).
+rewrite kron_plus_distr_l.
+rewrite Mmult_plus_distr_l.
+repeat rewrite Mmult_plus_distr_r.
+assert (Main1 : swapac × (∣0⟩⟨0∣ ⊗ I 4) × swapac = I 4 ⊗ ∣0⟩⟨0∣).
 {
-  set (A := ∣0⟩ × ∣0⟩†).
-  assert (Isplit : I 4 == I 2 ⊗ I 2). lma.
-  rewrite Isplit.
-  rewrite <- kron_assoc_mat.
-  apply a8_c.
+  set (A := ∣0⟩⟨0∣).
+  assert (A ⊗ I 4 = (A ⊗ I 2) ⊗ I 2). lma'.
+  rewrite H.
+  rewrite swapac_3q. 4: apply WF_I. 3: apply WF_I. 2: apply WF_braqubit0.
+  rewrite kron_I. 3: lia. 2: lia.
+  reflexivity.
 }
-rewrite Main1.
+rewrite Main1 at 1.
 rewrite <- Mplus_assoc.
-assert (Main2 : SWAPAC × (∣ 1 ⟩ × (∣ 1 ⟩) † ⊗ (∣ 0 ⟩ × (∣ 0 ⟩) † ⊗ I 2)) 
-× SWAPAC == I 2 ⊗ (∣0⟩ × ∣0⟩†) ⊗ (∣1⟩ × ∣1⟩†)).
+assert (Main2 : swapac × (∣1⟩⟨1∣ ⊗ (∣0⟩⟨0∣ ⊗ I 2)) × swapac =
+I 2  ⊗ ∣0⟩⟨0∣ ⊗ ∣1⟩⟨1∣).
 {
-  set (A := ∣0⟩ × ∣0⟩†).
-  set (B := ∣1⟩ × ∣1⟩†).
-  rewrite <- kron_assoc_mat.
-  apply a8_c.
+  set (A := ∣0⟩⟨0∣).
+  set (B := ∣1⟩⟨1∣).
+  rewrite <- kron_assoc. 4: apply WF_I. 3: apply WF_braqubit0. 2: apply WF_braqubit1.
+  apply swapac_3q. 3: apply WF_I. 2: apply WF_braqubit0. apply WF_braqubit1.
 }
-rewrite Main2.
-assert (Main3 : SWAPAC × (∣ 1 ⟩ × (∣ 1 ⟩) † ⊗ (∣ 1 ⟩ × (∣ 1 ⟩) † ⊗ Diag2 1 c1)) 
-× SWAPAC == Diag2 1 c1 ⊗ (∣1⟩ × ∣1⟩†) ⊗ (∣1⟩ × ∣1⟩†)).
+rewrite Main2 at 1.
+assert (Main3 : swapac × (∣1⟩⟨1∣ ⊗ (∣1⟩⟨1∣ ⊗ diag2 C1 c1)) × swapac =
+diag2 C1 c1 ⊗ ∣1⟩⟨1∣ ⊗ ∣1⟩⟨1∣).
 {
-  set (A := ∣1⟩ × ∣1⟩†).
-  set (B := Diag2 1 c1).
-  rewrite <- kron_assoc_mat.
-  apply a8_c.
+  set (A := ∣1⟩⟨1∣).
+  set (B := diag2 1 c1).
+  rewrite <- kron_assoc. 4: apply WF_diag2. 3: apply WF_braqubit1. 2: apply WF_braqubit1.
+  apply swapac_3q. 3: apply WF_diag2. 2: apply WF_braqubit1. apply WF_braqubit1.
 }
-rewrite Main3.
-lma.
-Qed. *)
+rewrite Main3 at 1.
+lma'. 2: solve_WF_matrix. 1: solve_WF_matrix.
+apply WF_diag2. apply WF_diag2.
+Qed.
