Vectors.v
@@ -1,0 +1,161 @@
+Require Import QuantumLib.Matrix.
+Require Import QuantumLib.Quantum.
+Require Import QuantumLib.VectorStates.
+From Proof Require Import QubitHelpers.
+
+Lemma a14 : forall (psi : Vector 4), 
+WF_Matrix psi -> ⟨ psi , psi ⟩ = 1 -> 
+exists (beta beta_p gamma gamma_p: Vector 2) (r : R)
+(* (WF_b : WF_Matrix beta) (WF_bp : WF_Matrix beta_p) (WF_g: WF_Matrix gamma) (WF_gp : WF_Matrix gamma_p) *),
+⟨ beta , beta_p ⟩ = 0 /\ ⟨ gamma , gamma_p ⟩ = 0 /\
+psi = √ (r) .* (beta ⊗ gamma) .+ √ (1-r) .* (beta_p ⊗ gamma_p).
+intros.
+Admitted.
+
+(* Definition of lemma from old file Multiqubit*)
+Lemma qubit_decomposition2 : forall (phi : Vector 4), 
+WF_Matrix phi -> exists (a b c d: C),
+phi = a .* ∣0,0⟩ .+ b .* ∣0,1⟩ .+ c .* ∣1,0⟩ .+ d .* ∣1,1⟩.
+Proof.
+  intros.
+  exists (phi 0 0)%nat, (phi 1 0)%nat, (phi 2 0)%nat, (phi 3 0)%nat.
+  lma'.
+  apply WF_plus. apply WF_plus. apply WF_plus.
+  apply WF_scale. apply WF_kron. reflexivity. reflexivity. apply WF_qubit0. apply WF_qubit0.
+  apply WF_scale. apply WF_kron. reflexivity. reflexivity. apply WF_qubit0. apply WF_qubit1.
+  apply WF_scale. apply WF_kron. reflexivity. reflexivity. apply WF_qubit1. apply WF_qubit0.
+  apply WF_scale. apply WF_kron. reflexivity. reflexivity. apply WF_qubit1. apply WF_qubit1.
+Qed.
+
+Property is_unitary_form : forall (M : Square 2) (a b : Vector 2), 
+  WF_Qubit a -> WF_Qubit b ->
+  M = a ⊗ ⟨0∣ .+ b ⊗ ⟨1∣ /\ ⟨a, b⟩ = 0 -> WF_Unitary M.
+Proof.
+  intros.
+  destruct H1 as [H1 H2].
+  rewrite H1.
+  destruct H as [_ [H WF_a]].
+  destruct H0 as [_ [H0 WF_b]].
+  rewrite qubit_adj_mult in WF_a. 2: apply H.
+  rewrite qubit_adj_mult in WF_b. 2: apply H0.
+  unfold WF_Unitary.
+  split. 
+  {
+    apply WF_plus.
+    apply WF_kron. reflexivity. reflexivity. apply H. apply WF_adjoint. apply WF_qubit0.
+    apply WF_kron. reflexivity. reflexivity. apply H0. apply WF_adjoint. apply WF_qubit1.
+  }
+  rewrite Mplus_adjoint.
+  rewrite (kron_adjoint a ⟨0∣).
+  rewrite (kron_adjoint b ⟨1∣).
+  repeat rewrite adjoint_involutive.
+  rewrite Mmult_plus_distr_l.
+  repeat rewrite Mmult_plus_distr_r.
+  rewrite (kron_mixed_product a† ∣0⟩ a ⟨0∣).
+  rewrite WF_a.
+  rewrite kron_1_l with (A := ∣0⟩⟨0∣). 2: apply WF_braqubit0.
+  rewrite (kron_mixed_product b† ∣1⟩ a ⟨0∣).
+  unfold inner_product in H2.
+  assert (Main1 : a† × b = b† × a).
+  {
+    lma'.
+    rewrite H2.
+    apply (f_equal (fun f => f^*)) in H2.
+    assert (Help : ((a† × b) 0%nat 0%nat)^* = ((b† × a) 0%nat 0%nat)). lca.
+    rewrite Help in H2.
+    rewrite Cconj_0 in H2.
+    symmetry.
+    apply H2.
+  }
+  rewrite <- Main1.
+  assert (Main2 : a† × b = Zero).
+  {
+    lma'.
+    apply H2.
+  }
+  rewrite Main2.
+  rewrite kron_0_l.
+  rewrite Mplus_0_r.
+  rewrite (kron_mixed_product a† ∣0⟩ b ⟨1∣).
+  rewrite Main2.
+  rewrite kron_0_l.
+  rewrite Mplus_0_l.
+  rewrite (kron_mixed_product b† ∣1⟩ b ⟨1∣).
+  rewrite WF_b.
+  lma'.
+Qed.
+
+Lemma a15 : forall (beta beta_p : Vector 2) (w : Vector 4), 
+WF_Qubit beta -> WF_Qubit beta_p -> WF_Qubit w -> 
+⟨beta, beta_p⟩ = 0 -> exists (psi phi : Vector 2), w = beta ⊗ psi .+ beta_p ⊗ phi.
+Proof.
+intros. 
+set (Q := beta ⊗ ⟨0∣ .+ beta_p ⊗ ⟨1∣).
+assert (WF_Q : WF_Unitary Q).
+{
+  apply is_unitary_form with (a := beta) (b := beta_p).
+  apply H. apply H0.
+  split.
+  unfold Q. reflexivity.
+  apply H2.
+}
+assert (HQ_impl := qubit_decomposition2 ((Q ⊗ I 2)† × w)).
+assert (WF_QI2 : WF_Matrix (Q ⊗ I 2)). 
+{
+  apply WF_kron. reflexivity. reflexivity. apply WF_Q. apply WF_I.
+}
+assert (HQ: WF_Matrix ((Q ⊗ I 2) † × w)). 
+{
+  apply WF_mult. apply WF_adjoint. apply WF_QI2.
+  apply H1.
+}
+apply HQ_impl in HQ.
+destruct HQ as [c00 [c01 [c10 [c11 HQ]]]].
+repeat rewrite <- Mscale_kron_dist_r in HQ.
+rewrite <- kron_plus_distr_l in HQ.
+rewrite Mplus_assoc in HQ.
+rewrite <- kron_plus_distr_l in HQ.
+rewrite <- ket0_equiv in HQ.
+rewrite <- ket1_equiv in HQ.
+set (psi := c00 .* ∣0⟩ .+ c01 .* ∣1⟩).
+set (phi := c10 .* ∣0⟩ .+ c11 .* ∣1⟩).
+assert (WF_psi: WF_Matrix psi).
+{
+  apply WF_plus. apply WF_scale. apply WF_qubit0. apply WF_scale. apply WF_qubit1.
+}
+assert (WF_phi: WF_Matrix phi).
+{
+  apply WF_plus. apply WF_scale. apply WF_qubit0. apply WF_scale. apply WF_qubit1.
+}
+fold psi in HQ. fold phi in HQ.
+exists psi, phi.
+assert (Step1: beta ⊗ psi .+ beta_p ⊗ phi = (Q ⊗ I 2) × (∣0⟩ ⊗ psi .+ ∣1⟩ ⊗ phi)).
+{
+  lma'.
+  apply WF_plus. 
+  apply WF_kron. reflexivity. reflexivity. apply H.
+  apply WF_psi.
+  apply WF_kron. reflexivity. reflexivity. apply H0.
+  apply WF_phi.
+
+}
+rewrite Step1.
+rewrite <- HQ.
+rewrite <- Mmult_assoc.
+assert (WF_QI : WF_Unitary (Q ⊗ I 2)†).
+{
+  apply transpose_unitary.
+  apply kron_unitary.
+  apply WF_Q.
+  apply id_unitary.
+}
+destruct WF_QI as [_ WF_QI].
+rewrite adjoint_involutive in WF_QI.
+rewrite WF_QI at 1.
+rewrite Mmult_1_l. 2: apply H1.
+reflexivity.
+Qed.
+
+Definition linearly_independent_2vec {n} (v1 v2 : Vector n) := 
+  forall (c1 c2 : C), c1 .* v1 .+ c2 .* v2 = Zero -> c1 = 0 /\ c2=0.
+
